Tables/Table/Raw.lean
@@ -4,3 +4,4 @@ public import Tables.Table.Raw.Basic
 public import Tables.Table.Raw.BasicLemmas
 public import Tables.Table.Raw.Join
 public import Tables.Table.Raw.JoinLemmas
+public import Tables.Table.Raw.Sort
